spongeScript.sml
@@ -1,0 +1,779 @@
+
+(**********************************************************************)
+(* Formalization of sponge function using an arbitrary permutation    *)
+(**********************************************************************)
+
+(**********************************************************************
+
+Roughly:
+
+ Hash msg =  Output(Absorb initial_state (Split (Pad msg)))
+
+  - Pad adds additional bits (specified by Keccak) to 
+    extend msg so the result can be split into blocks
+
+  - Split splits a message into a list of blocks
+
+  - Absorb applies the sponge algorithm, starting from initial_state
+
+  - Outputs extracts the digest from the state resulting from absorbing
+
+More precisely, the algorithm is parametrised over a permutation f,
+used for absorbing, and (r,c,n) where r is the "bitrate" (i.e. block
+size), c is the "capacity" (a parameter used by the sponge algorithm)
+and n is the digest length. The definition of Hash is thus actually:
+
+ Hash (r,c,n) f initial_state msg = 
+  Output n (Absorb f c initial_state (Split r (Pad r msg)))
+
+The initial_state consists entirely of zeros.
+
+***********************************************************************) 
+
+(* Load stuff below when running interactively *)
+
+(*
+app load ["rich_listTheory","intLib","Cooper"];
+open HolKernel Parse boolLib bossLib
+     listTheory rich_listTheory 
+     arithmeticTheory Arith numLib computeLib
+     Cooper;
+
+intLib.deprecate_int();
+*)
+
+
+(* Hide stuff above and expose stuff below when compiling *)
+open HolKernel Parse boolLib bossLib
+     listTheory rich_listTheory 
+     arithmeticTheory Arith numLib computeLib
+     wordsLib
+     Cooper;
+
+val _ = intLib.deprecate_int();
+
+(**********************************************************************)
+(* Start new theory MITB_SPEC                                         *)
+(**********************************************************************)
+
+val _ = new_theory "sponge";
+
+(* 
+Bit sizes:
+ digest   (n): 224
+ capacity (c): 448
+ bitrate  (r): 1152 (block and key size)
+ width    (b): 1600 (SHA-3 state size = r+c)
+*)
+
+(*
+Started using wordLib for bit-strings, but switched to using lists of
+Booleans because symbolic execution was simpler. Might switch back to
+wordsLib later.
+*)
+
+(*
+List of zeros (represented as Fs) of a given size
+*)
+
+val _ = type_abbrev("bits", ``:bool list``);
+
+val Zeros_def =
+ Define
+  `(Zeros 0 = [])
+   /\
+   (Zeros(SUC n) = F :: Zeros n)`;
+
+val WORD_TO_BITS_def=
+  Define
+  ` WORD_TO_BITS (w:'l word) =
+  let 
+    bitstring_without_zeros =  MAP (\e.if e=1 then T else F) (word_to_bin_list w)
+  in
+    ( Zeros (dimindex(:'l) - (LENGTH bitstring_without_zeros) )) ++
+    bitstring_without_zeros`;
+
+val BITS_TO_WORD_def=
+  Define
+  ` BITS_TO_WORD = 
+      word_from_bin_list o ( MAP (\e.if e=T then 1 else 0))`;
+
+
+
+(*
+Sanity checks
+*)
+val LengthZeros =
+ store_thm
+  ("LengthZeros",
+   ``!n. LENGTH(Zeros n) = n``,
+   Induct
+    THEN RW_TAC list_ss [Zeros_def]);
+
+val ZerosOneToOne =
+ store_thm
+  ("ZerosOneToOne",
+   ``!m n. (Zeros m = Zeros n) = (m = n)``,
+   Induct 
+    THEN Induct
+    THEN RW_TAC list_ss [Zeros_def]);
+
+(*        
+PadZeros r msg computes the smallest number n such that the length of
+(msg ++ [T] ++ Zeros n ++ [T]) is a multiple of r, i.e.:
+
+ LENGTH(msg ++ [T] ++ Zeros n ++ [T]) MOD r = 0
+
+The theorem names LeastPad, proved below, verifies that PadZeros
+has this property:
+
+ LeastPad
+ |- !r msg.
+     2 < r 
+     ==>
+     (LENGTH (msg ++ [T] ++ Zeros (PadZeros r msg) ++ [T]) MOD r = 0) 
+     /\
+     !n. (LENGTH (msg ++ [T] ++ Zeros n ++ [T]) MOD r = 0) 
+         ==>
+         PadZeros r msg <= n
+
+Robert's definition of PadZeros is used below. This is:
+
+ |- PadZeros r msg = (r - ((LENGTH msg + 2) MOD r)) MOD r
+
+The theorem PadZerosLemma, proved below, verifies an alterntive
+definition:
+
+ PadZerosLemma
+ |- !msg r.
+     1 < r
+     ==> 
+     (PadZeros r msg = 
+       if (LENGTH msg MOD r = r - 1 )
+        then r - 1
+        else r - LENGTH msg MOD r - 2)
+
+*)
+val PadZeros_def =
+ Define
+  `PadZeros r msg = (r - ((LENGTH msg + 2) MOD r)) MOD r`;
+
+(*
+Pad r msg adds Keccak padding to msg. The theorem LengthPadDivides
+proved below verifies:
+
+ LengthPadDivides
+ |- !r msg. 2 < r ==> (LENGTH(Pad r msg) MOD r = 0)
+*)
+val Pad_def =
+ Define
+  `Pad r msg = msg ++ [T] ++ Zeros(PadZeros r msg) ++ [T]`;
+
+(* 
+Various lemmas needed to prove LeastPad, PadZerosLemma and
+LengthPadDivides.
+
+The HOL4 proofs could probably be made much shorter and more elegant
+(I just mechanically blundered through them)
+*)
+
+val LengthPadLemma1 =
+ prove
+  (``!r msg n. 
+      (2 < r) /\ (LENGTH msg = n * r) 
+      ==> 
+      (LENGTH(Pad r msg) = (n + 1) * r)``,
+   RW_TAC list_ss [Pad_def,PadZeros_def,LengthZeros,MOD_TIMES]);
+
+val MOD_SUB_MOD =
+ prove
+  (``!m n r. 0 < r /\ 0 < n MOD r ==> ((r - n MOD r) MOD r = r - n MOD r)``,
+   RW_TAC arith_ss []);
+
+val MULT_ADD_MOD =
+ prove
+  (``!n p r. p < r ==> ((n * r + p) MOD r = p)``,
+   RW_TAC arith_ss[]
+    THEN `0 < r` by DECIDE_TAC
+    THEN PROVE_TAC[MOD_TIMES,ADD_SYM,LESS_MOD]);
+   
+val LengthPadLemma2 =
+ prove
+  (``!r msg n p. 
+      (0 < p) /\ (p + 2 < r) /\ (LENGTH msg = n * r + p) 
+      ==> 
+      (LENGTH(Pad r msg) = (n + 1) * r)``,
+   RW_TAC list_ss [Pad_def,PadZeros_def,LengthZeros,MOD_TIMES]
+    THEN `0 < p + 2` by DECIDE_TAC
+    THEN `p + (n * r + 2) = n * r + (p + 2)` by PROVE_TAC[ADD_SYM,ADD_ASSOC]
+    THEN `0 < (n * r + (p + 2)) MOD r` by PROVE_TAC[MULT_ADD_MOD]
+    THEN `p < r` by DECIDE_TAC
+    THEN `0 < r` by DECIDE_TAC
+    THEN RW_TAC std_ss [MOD_SUB_MOD,MULT_ADD_MOD]
+    THEN DECIDE_TAC);
+
+val LengthPadLemma3 =
+ prove
+  (``!r msg n. 
+      (2 < r) /\ (LENGTH msg = n * r + (r - 2)) 
+      ==> 
+      (LENGTH(Pad r msg) = (n + 1) * r)``,
+   RW_TAC list_ss [Pad_def,PadZeros_def,LengthZeros,MOD_TIMES]
+    THEN `r + n * r = (n + 1) * r` by DECIDE_TAC
+    THEN `0 < r` by DECIDE_TAC
+    THEN RW_TAC std_ss [MOD_EQ_0]
+    THEN RW_TAC arith_ss []);
+
+val LengthPadLemma4 =
+ prove
+  (``!r msg n. 
+      (2 < r) /\ (LENGTH msg = n * r + (r - 1)) 
+      ==> 
+      (LENGTH(Pad r msg) = (n + 2) * r)``,
+   RW_TAC list_ss [Pad_def,PadZeros_def,LengthZeros,MOD_TIMES]
+    THEN `r + (n * r + 1) = (n + 1) * r + 1` 
+          by PROVE_TAC[ADD_SYM,ADD_ASSOC,RIGHT_ADD_DISTRIB,MULT_LEFT_1]
+    THEN RW_TAC std_ss []
+    THEN `1 < r` by DECIDE_TAC
+    THEN RW_TAC std_ss [MULT_ADD_MOD]
+    THEN `r - 1 < r` by DECIDE_TAC
+    THEN RW_TAC std_ss [LESS_MOD]
+    THEN DECIDE_TAC);
+
+val LengthPadLemma5 =
+ prove
+  (``!r msg n p. 
+      2 < r /\ p < r /\ (LENGTH msg = n * r + p) 
+      ==> 
+      (LENGTH(Pad r msg) = (n + (if p = r - 1 then 2 else 1)) * r)``,
+   RW_TAC std_ss []
+    THENL
+     [PROVE_TAC[LengthPadLemma4],
+      Cases_on `0 < p`
+       THENL
+        [`p + 2 < r \/ (p = r - 2) \/ (p = r - 1)`
+          by PROVE_TAC
+              [DECIDE 
+                ``2 < r /\ p < r ==> p + 2 < r \/ (p = r - 2) \/ (p = r - 1)``]
+          THENL
+           [PROVE_TAC[LengthPadLemma2],
+            PROVE_TAC[LengthPadLemma3]],
+         `p = 0` by DECIDE_TAC
+          THEN RW_TAC arith_ss []
+          THEN `LENGTH msg = n * r` by PROVE_TAC[ADD_0]
+          THEN IMP_RES_TAC LengthPadLemma1
+          THEN DECIDE_TAC]]);
+
+val LengthPadLemma6 =
+ prove
+  (``!r msg. 
+      2 < r 
+      ==> 
+      ?n p.
+       p < r
+       /\
+       (LENGTH msg = n*r + p)
+       /\
+       (LENGTH(Pad r msg) = if p = r-1 then (n+2)*r else (n+1)*r)``,
+   RW_TAC std_ss []
+    THEN `?n p. (LENGTH msg = n * r + p) /\ p < r`
+          by PROVE_TAC[DIVISION, DECIDE ``2<r ==> 0<r``]
+    THEN Q.EXISTS_TAC `n`
+    THEN Q.EXISTS_TAC `p`
+    THEN RW_TAC std_ss []
+    THEN IMP_RES_TAC LengthPadLemma5
+    THEN RW_TAC std_ss []);
+
+(*
+Pad r msg produces a strin whose length is a multiple of r
+*)
+val LengthPad =
+ store_thm
+  ("LengthPad",
+   ``!r msg. 
+      2 < r 
+      ==> 
+      (LENGTH(Pad r msg) = 
+        (if (LENGTH msg MOD r) = r-1 
+          then ((LENGTH msg DIV r) + 2) 
+          else ((LENGTH msg DIV r) + 1)) * r)``,
+   RW_TAC std_ss []
+    THEN IMP_RES_TAC LengthPadLemma6
+    THEN POP_ASSUM(STRIP_ASSUME_TAC o SPEC ``msg : bool list``)
+    THEN PROVE_TAC[DIV_UNIQUE,MOD_UNIQUE]);
+
+val LengthPadDivides =
+ store_thm
+  ("LengthPadDivides",
+   ``!r msg. 2 < r ==> (LENGTH(Pad r msg) MOD r = 0)``,
+   RW_TAC std_ss []
+    THEN `0 < r` by DECIDE_TAC
+    THEN RW_TAC std_ss [LengthPad,MOD_EQ_0]);
+
+(*
+More lemmas needed for proving that minimal padding added
+*)
+val ADD_MOD_ZERO1 =
+ prove
+  (``!m p r.
+      0 < r /\ ((m + p) MOD r = 0)
+      ==>
+      ?n. p = n * r - m MOD r``,
+   RW_TAC arith_ss []
+    THEN `?d. m + p = d * r` by PROVE_TAC[MOD_EQ_0_DIVISOR]
+    THEN `((m DIV r) * r + m MOD r + p = d * r) /\ m MOD r < r` 
+          by PROVE_TAC[DIVISION]
+    THEN Q.EXISTS_TAC `d - (m DIV r)`
+    THEN RW_TAC arith_ss [RIGHT_SUB_DISTRIB]);
+
+val ADD_MOD_ZERO1_COR =
+ prove
+  (``!m p r.
+      0 < r /\ 0 < p /\ ((m + p) MOD r = 0)
+      ==>
+      ?n. 0 < n /\ (p = n * r - m MOD r)``,
+   RW_TAC std_ss []
+    THEN IMP_RES_TAC ADD_MOD_ZERO1
+    THEN POP_ASSUM(K ALL_TAC)
+    THEN Cases_on `n=0`
+    THEN RW_TAC arith_ss []
+    THEN `0 < n` by DECIDE_TAC
+    THEN PROVE_TAC[]);
+
+val ADD_MOD_ZERO2 =
+ prove
+  (``!m p r.
+      0 < r /\ (?n. 0 < n /\ (p = n * r - m MOD r))
+      ==>
+      ((m + p) MOD r = 0)``,
+   RW_TAC arith_ss []
+    THEN `(m = (m DIV r) * r + m MOD r) /\ m MOD r < r` 
+          by PROVE_TAC[DIVISION]
+    THEN `n = SUC(PRE n)` by DECIDE_TAC
+    THEN POP_ASSUM(ASSUME_TAC o SIMP_RULE arith_ss [ADD1])
+    THEN POP_ASSUM(fn th => SUBST_TAC[th])
+    THEN RW_TAC arith_ss [RIGHT_ADD_DISTRIB]
+    THEN `(m + (r + r * PRE n) - m MOD r) = m DIV r * r + r + r * PRE n`
+          by DECIDE_TAC
+    THEN RW_TAC std_ss []
+    THEN `m DIV r * r + r + r * PRE n = m DIV r * r + 1 * r + PRE n * r`
+          by PROVE_TAC[MULT_SYM,MULT_LEFT_1]
+    THEN ONCE_ASM_REWRITE_TAC[]
+    THEN PROVE_TAC[MOD_EQ_0,RIGHT_ADD_DISTRIB]);
+
+val ADD_MOD_ZERO =
+ prove
+  (``!m p r.
+      0 < r /\ 0 < p
+      ==>
+     (((m + p) MOD r = 0) =
+      ?n. 0 < n /\ (p = n * r - m MOD r))``,
+   RW_TAC arith_ss []
+    THEN EQ_TAC
+    THENL
+     [PROVE_TAC[ADD_MOD_ZERO1_COR],
+      PROVE_TAC[ADD_MOD_ZERO2]]);
+
+val ADD_MOD_ZERO_COR1 =
+ prove
+  (``!msg n r.
+      0 < r
+      ==>
+     ((LENGTH(msg ++ [T] ++ Zeros n ++ [T]) MOD r = 0) =
+      ?m. 0 < m /\ (n + 2 = m * r - LENGTH msg MOD r))``,
+   RW_TAC list_ss [LengthZeros]
+    THEN PROVE_TAC
+          [DECIDE ``0 < n+2 /\ (m + (n + 2) = n + (m + 2))``,
+           ADD_MOD_ZERO]);
+
+val ADD_MOD_ZERO_COR2 =
+ prove
+  (``!msg n r.
+      2 < r
+      ==>
+     ((LENGTH(msg ++ [T] ++ Zeros n ++ [T]) MOD r = 0) =
+      ?m. (if LENGTH msg MOD r = r - 1 then 1 else 0) < m
+          /\ 
+          (n = m * r - LENGTH msg MOD r - 2))``,
+   RW_TAC std_ss []
+    THEN `0 < r` by DECIDE_TAC
+    THEN RW_TAC std_ss [ADD_MOD_ZERO_COR1]
+    THENL
+     [EQ_TAC
+       THENL
+        [RW_TAC std_ss []
+          THEN Cases_on `m = 1`
+          THEN RW_TAC arith_ss []
+          THEN `?m'. m = m' + 2` by COOPER_TAC
+          THEN `?r'. r = r' + 3` by COOPER_TAC
+          THEN FULL_SIMP_TAC arith_ss [LEFT_ADD_DISTRIB,RIGHT_ADD_DISTRIB]
+          THEN `n = 3 * m' + (r' + (m' * r' + 4)) - 2` by DECIDE_TAC
+          THEN RW_TAC arith_ss []
+          THEN Q.EXISTS_TAC `2+m'`
+          THEN RW_TAC arith_ss [],
+         RW_TAC std_ss []
+          THEN `?m'. m = m' + 2` by COOPER_TAC
+          THEN RW_TAC std_ss [RIGHT_ADD_DISTRIB]
+          THEN Q.EXISTS_TAC `m'+2`
+          THEN RW_TAC arith_ss []],
+      `LENGTH msg MOD r < r` by PROVE_TAC[MOD_LESS]
+       THEN `LENGTH msg MOD r < r-1` by DECIDE_TAC
+       THEN EQ_TAC
+       THEN RW_TAC std_ss []
+       THEN`?m'. m = m' + 1` by COOPER_TAC
+       THEN FULL_SIMP_TAC arith_ss [LEFT_ADD_DISTRIB,RIGHT_ADD_DISTRIB]
+       THEN Q.EXISTS_TAC `m'+1`
+       THEN RW_TAC arith_ss []]);
+
+val MOD_ADD2_EQ =
+ prove
+  (``!m r. 1 < r /\ (m MOD r = r - 1) ==> ((m + 2) MOD r = 1)``,
+   RW_TAC arith_ss []
+    THEN `0 < r` by DECIDE_TAC
+    THEN `m = m DIV r * r + (r - 1)` by PROVE_TAC[DIVISION]
+    THEN POP_ASSUM(fn th => SUBST_TAC[th])
+    THEN `m DIV r * r + (r - 1) + 2 = m DIV r * r + (r + 1)`
+          by DECIDE_TAC
+    THEN RW_TAC std_ss [MOD_TIMES]
+    THEN PROVE_TAC[MULT_LEFT_1,MULT_ADD_MOD]);
+
+val MOD_ADD2_NEQ =
+ prove
+  (``!m r.
+      1 < r /\ m MOD r <> r - 1 ==>
+      ((r - (m + 2) MOD r) MOD r = r - m MOD r - 2)``,
+   RW_TAC arith_ss []
+    THEN `0 < r` by DECIDE_TAC
+    THEN `m MOD r < r` by PROVE_TAC[MOD_LESS]
+    THEN `m MOD r < r - 1` by DECIDE_TAC
+    THEN `m = m DIV r * r + m MOD r` by PROVE_TAC[DIVISION]
+    THEN POP_ASSUM(fn th => SUBST_TAC[th])
+    THEN `m DIV r * r + m MOD r + 2 = m DIV r * r + (m MOD r + 2)` by DECIDE_TAC
+    THEN RW_TAC std_ss [MOD_TIMES]
+    THEN Cases_on `m MOD r + 2 = r`
+    THEN RW_TAC arith_ss []);
+
+val PadZerosLemma1 =
+ prove
+  (``!r msg.
+      1 < r /\ (LENGTH msg MOD r = r - 1) 
+      ==> 
+      (PadZeros r msg = r - 1)``,
+   RW_TAC arith_ss [PadZeros_def,MOD_ADD2_EQ]);
+
+val PadZerosLemma2 =
+ prove
+  (``!r msg.
+      1 < r /\ ~(LENGTH msg MOD r = r - 1) 
+      ==> 
+      (PadZeros r msg = r - LENGTH msg MOD r - 2)``,
+   REWRITE_TAC[PadZeros_def,MOD_ADD2_NEQ]);
+
+val PadZerosLemma =
+ store_thm
+ ("PadZerosLemma",
+  ``!r msg.
+     1 < r
+     ==> 
+     (PadZeros r msg = 
+       if (LENGTH msg MOD r = r - 1 )
+        then r - 1
+        else r - LENGTH msg MOD r - 2)``,
+  RW_TAC arith_ss [PadZerosLemma1,PadZerosLemma2]);
+
+val LeastPad1 =
+ prove
+  (``!r msg.
+      2 < r /\ (LENGTH msg MOD r = r - 1 ) 
+      ==> (LENGTH(msg ++ [T] ++ Zeros(r - 1) ++ [T]) MOD r = 0)``,
+   RW_TAC std_ss []
+    THEN `0 < r` by DECIDE_TAC
+    THEN `1 < r` by DECIDE_TAC
+    THEN `r - 1 = PadZeros r msg` by PROVE_TAC[PadZerosLemma]
+    THEN RW_TAC arith_ss [GSYM Pad_def,LengthPad]
+    THEN PROVE_TAC[MOD_EQ_0,MULT_SYM]);
+
+val LeastPad2 =
+ prove
+  (``!r msg.
+      2 < r 
+      /\ 
+      (LENGTH msg MOD r = r - 1 ) 
+      /\
+      (LENGTH(msg ++ [T] ++ Zeros n ++ [T]) MOD r = 0)
+      ==>
+      r - 1 <= n``,
+   RW_TAC std_ss []
+    THEN `?m. 1 < m /\ (n = m * r - LENGTH msg MOD r - 2)`
+          by PROVE_TAC[ADD_MOD_ZERO_COR2]
+    THEN `?m'. m = m' + 2` by COOPER_TAC
+    THEN RW_TAC std_ss [RIGHT_ADD_DISTRIB]
+    THEN DECIDE_TAC);
+
+val LeastPad3 =
+ prove
+  (``!r msg. 
+      2 < r /\ ~(LENGTH msg MOD r = r - 1 ) 
+      ==> 
+      (LENGTH(msg ++ [T] ++ Zeros(r - LENGTH msg MOD r - 2) ++ [T]) MOD r = 0)``,
+   RW_TAC std_ss []
+    THEN `0 < r` by DECIDE_TAC
+    THEN `1 < r` by DECIDE_TAC
+    THEN `r - LENGTH msg MOD r - 2 = PadZeros r msg` 
+          by PROVE_TAC[PadZerosLemma]
+    THEN RW_TAC arith_ss [GSYM Pad_def,LengthPad]
+    THEN PROVE_TAC[MOD_EQ_0,MULT_SYM]);
+
+val LeastPad4 =
+ prove
+  (``!r msg.
+      2 < r 
+      /\ 
+      ~(LENGTH msg MOD r = r - 1 ) 
+      /\
+      (LENGTH(msg ++ [T] ++ Zeros n ++ [T]) MOD r = 0)
+      ==>
+      r - LENGTH msg MOD r - 2 <= n``,
+   RW_TAC std_ss []
+    THEN `?m. 0 < m /\ (n = m * r - LENGTH msg MOD r - 2)`
+          by PROVE_TAC[ADD_MOD_ZERO_COR2]
+    THEN `?m'. m = m' + 1` by COOPER_TAC
+    THEN FULL_SIMP_TAC std_ss [RIGHT_ADD_DISTRIB]
+    THEN DECIDE_TAC);
+
+(*
+Proof that PadZeros r msg computes the smallest number n such that the
+length of (msg ++ [T] ++ Zeros n ++ [T]) is a multiple of r, i.e.:
+*)
+val LeastPad =
+ store_thm
+  ("LeastPad",
+   ``!r msg.
+      2 < r 
+      ==>
+      (LENGTH(msg ++ [T] ++ Zeros(PadZeros r msg) ++ [T]) MOD r = 0)
+      /\
+      !n. (LENGTH(msg ++ [T] ++ Zeros n ++ [T]) MOD r = 0)
+          ==>
+          PadZeros r msg <= n``,
+   REPEAT GEN_TAC THEN DISCH_TAC
+    THEN `1 < r` by DECIDE_TAC
+    THEN Cases_on `LENGTH msg MOD r = r - 1`
+    THEN RW_TAC pure_ss [PadZerosLemma]
+    THEN RW_TAC std_ss [LeastPad1,LeastPad2,LeastPad3,LeastPad4]
+    THEN `r - 1 <= n` by PROVE_TAC[LeastPad2]
+    THEN DECIDE_TAC);
+
+(*
+Split a message into blocks of a given length r, with the last block
+being shorter if the r doesn't divide exactly into the block length.
+*)
+val Split_def =
+ tDefine
+  "Split"
+  `Split r msg = 
+    if (r = 0) \/ LENGTH msg <= r 
+     then [msg]
+     else TAKE r msg :: Split r (DROP r msg)`
+  (WF_REL_TAC `measure (LENGTH o SND)`
+    THEN RW_TAC list_ss [LENGTH_DROP]);
+
+
+val Split_ind = (fetch "-" "Split_ind");
+
+(*
+Sanity check:
+
+ - each block has length shorter than r;
+
+ - if there are more than one blocks in a message, 
+   then all except the last have length r;
+
+ - the concatenation of the blocks is the original message.
+
+The first two of these are verified by the theorem:
+
+ SplitBlockLengths
+ |- !r msg.
+     0 < r ==>
+     LENGTH (EL (PRE (LENGTH (Split r msg))) (Split r msg)) <= r /\
+     !n.
+       n < PRE (LENGTH (Split r msg)) ==>
+       (LENGTH (EL n (Split r msg)) = r)
+
+and the third property by:
+
+ FlattenSplit
+ |- !r msg. 0 < r ==> (FLAT (Split r msg) = msg)
+
+Note that EL ((LENGTH l) - 1) l = LAST l as shown by:
+
+ listTheory.LAST_EL (THEOREM)
+ |- !ls. ls <> [] ==> (LAST ls = EL (PRE (LENGTH ls)) ls)
+*)
+
+val SplitLengthsLemma1 =
+ prove
+  (``!r msg n. 
+      n < PRE(LENGTH(Split r msg))
+      ==> 
+      (LENGTH(EL n (Split r msg)) = r)``,
+   recInduct(fetch "-" "Split_ind")
+    THEN RW_TAC list_ss []
+    THEN RW_TAC list_ss [Once Split_def]
+    THENL
+     [`n < PRE (LENGTH [msg])` by PROVE_TAC[Split_def]
+       THEN FULL_SIMP_TAC list_ss [],
+      `n < PRE (LENGTH [msg])` by PROVE_TAC[Split_def]
+       THEN FULL_SIMP_TAC list_ss [],
+      Cases_on `n`
+       THEN RW_TAC list_ss []
+       THEN `n' < PRE (LENGTH (Split r (DROP r msg))) ==>
+             (LENGTH (EL n' (Split r (DROP r msg))) = r)` 
+             by PROVE_TAC[]
+       THEN `Split r msg = TAKE r msg::Split r (DROP r msg)` 
+             by PROVE_TAC[Split_def]
+       THEN FULL_SIMP_TAC list_ss []]);
+ 
+val SplitLengthsLemma2 =
+ prove
+  (``!r msg. 0 < LENGTH(Split r msg)``,
+   RW_TAC list_ss [Once Split_def]);
+
+val SplitLengthsLemma3 =
+ prove
+  (``!r msg.
+      0 < r
+      ==>
+      LENGTH(EL (PRE(LENGTH(Split r msg))) (Split r msg)) <= r``,
+   recInduct(fetch "-" "Split_ind")
+    THEN RW_TAC list_ss []
+    THEN RW_TAC list_ss [Once Split_def]
+    THENL
+     [`Split r msg = [msg]` by PROVE_TAC[Split_def]
+        THEN RW_TAC list_ss [],
+      `r <> 0` by DECIDE_TAC
+       THEN `LENGTH
+             (EL 
+               (PRE (LENGTH (Split r (DROP r msg)))) 
+               (Split r (DROP r msg))) <= r`
+             by PROVE_TAC[]
+       THEN `Split r msg = TAKE r msg::Split r (DROP r msg)` by PROVE_TAC[Split_def]
+       THEN `0 < (LENGTH (Split r (DROP r msg)))` by PROVE_TAC[SplitLengthsLemma2]
+       THEN RW_TAC list_ss [EL_CONS]]);
+
+val SplitBlockLengths =
+ store_thm
+  ("SplitBlockLengths",
+   ``!r msg.
+      0 < r
+      ==>
+      (LENGTH(EL (PRE(LENGTH(Split r msg))) (Split r msg)) <= r)
+      /\
+      (!n. n < PRE(LENGTH(Split r msg)) ==> (LENGTH(EL n (Split r msg)) = r))``,
+   PROVE_TAC[SplitLengthsLemma1,SplitLengthsLemma3]);
+
+val FlattenSplit =
+ prove
+  (``!r msg. 0 < r ==> (FLAT(Split r msg) = msg)``,
+   recInduct(fetch "-" "Split_ind")
+    THEN RW_TAC list_ss []
+    THEN RW_TAC list_ss [Once Split_def]);
+
+(* Sanity ckecking tests
+EVAL ``Split 4 (Pad 4 [m0;m1;m2;m3;m4;m5])``;
+EVAL ``Split 4 (Pad 4 [m0;m1;m2;m3;m4;m5;m6])``;
+EVAL ``Split 4 (Pad 4 [m0;m1;m2;m3;m4;m5;m6;m7])``;
+EVAL ``Split 4 (Pad 4 [m0;m1;m2;m3;m4;m5;m6;m7;m8])``;
+EVAL ``Split 4 (Pad 4 [m0;m1;m2;m3;m4;m5;m6;m7;m8;m9;m10])``;
+EVAL ``Split 4 (Pad 4 [m0;m1;m2;m3;m4;m5;m6;m7;m8;m9;m10;m11])``;
+EVAL ``Split 4 (Pad 4 [m0;m1;m2;m3;m4;m5;m6;m7;m8;m9;m10;m11;m12])``;
+EVAL ``Split 4 (Pad 4 [m0;m1;m2;m3;m4;m5;m6;m7;m8;m9;m10;m11;m12;m13])``;
+*)
+
+
+(*
+Absorb f c : state -> block list -> state
+*)
+val Absorb_def =
+ Define
+  `(Absorb f s ([]:'r word list)  = s)
+   /\
+   (Absorb f (s: ('r+'c) word) (blk::blkl) = 
+     Absorb f (f(s ?? (blk @@ 0w: 'c word))) blkl)`;
+
+(* Sanity check: relate Absorb to FOLDL *)
+val Absorb_FOLDL =
+ store_thm
+  ("Absorb_FOLDL",
+   ``Absorb (f: ('r+'c) word -> ('r+'c) word) = FOLDL (\s blk. f(s ?? (blk @@
+   (0w: 'c word))))``,
+   RW_TAC std_ss [FUN_EQ_THM] 
+    THEN Q.SPEC_TAC(`x`,`s0`)
+    THEN Q.SPEC_TAC(`x'`,`blkl`)
+    THEN Induct
+    THEN RW_TAC list_ss [Absorb_def]);
+
+(*
+Extract digest from a state
+*)
+val Output_def =
+ Define
+  `Output: ('b) word -> 'n word s =
+     ((dimindex(:'b)-1) >< (dimindex(:'b)-dimindex(:'n))) s`;
+
+val Split_words_def = 
+  Define
+  `SplittoWords: bits -> 'r word list =
+    (MAP BITS_TO_WORD) o (Split (dimindex(:'r)))`;
+
+(*
+Hash a message
+(('r+'c)word ->('r+'c)word) -> ('r+'c)word -> bits -> 'n word )
+*)
+val Hash_def =
+ Define
+  `Hash f initial_state  msg = 
+    Output (Absorb f initial_state 
+       (SplittoWords (Pad ( dimindex(:'r) ) msg)
+     : 'r word list  )
+       )`;
+
+(* Example 
+val (r,c,n) = (``4``,``2``,``3``);
+val s = ``Zeros(r+c)``;
+
+EVAL ``Hash (4,2,3) f ^s []``;
+EVAL ``Hash (4,2,3) f ^s [m0]``;
+EVAL ``Hash (4,2,3) f ^s [m0;m1]``;
+EVAL ``Hash (4,2,3) f ^s [m0;m1;m2]``;
+EVAL ``Hash (4,2,3) f ^s [m0;m1;m2;m3]``;
+EVAL ``Hash (4,2,3) f ^s [m0;m1;m2;m3;m4]``;
+EVAL ``Hash (4,2,3) f ^s [m0;m1;m2;m3;m4;m5]``;
+EVAL ``Hash (4,2,3) f ^s [m0;m1;m2;m3;m4;m5;m6]``;
+EVAL ``Hash (4,2,3) f ^s [m0;m1;m2;m3;m4;m5;m6;m7]``;
+EVAL ``Hash (4,2,3) f ^s [m0;m1;m2;m3;m4;m5;m6;m7;m8;m9]``;
+EVAL ``Hash (4,2,3) f ^s [m0;m1;m2;m3;m4;m5;m6;m7;m8;m9;m10]``;
+EVAL ``Hash (4,2,3) f ^s [m0;m1;m2;m3;m4;m5;m6;m7;m8;m9;m10;m11]``;
+*)
+
+(* Some test data:
+val (r,c,n) = (``4``,``2``,``3``);
+val s = ``Zeros(^r+^c)``;
+
+EVAL ``Hash (4,2,3) f ^s []``;
+EVAL ``Hash (4,2,3) f ^s [m0]``;
+EVAL ``Hash (4,2,3) f ^s [m0;m1]``;
+EVAL ``Hash (4,2,3) f ^s [m0;m1;m2]``;
+EVAL ``Hash (4,2,3) f ^s [m0;m1;m2;m3]``;
+EVAL ``Hash (4,2,3) f ^s [m0;m1;m2;m3;m4]``;
+EVAL ``Hash (4,2,3) f ^s [m0;m1;m2;m3;m4;m5]``;
+EVAL ``Hash (4,2,3) f ^s [m0;m1;m2;m3;m4;m5;m6]``;
+EVAL ``Hash (4,2,3) f ^s [m0;m1;m2;m3;m4;m5;m6;m7]``;
+EVAL ``Hash (4,2,3) f ^s [m0;m1;m2;m3;m4;m5;m6;m7;m8]``;
+EVAL ``Hash (4,2,3) f ^s [m0;m1;m2;m3;m4;m5;m6;m7;m8;m9]``;
+EVAL ``Hash (4,2,3) f ^s [m0;m1;m2;m3;m4;m5;m6;m7;m8;m9;m10]``;
+EVAL ``Hash (4,2,3) f ^s [m0;m1;m2;m3;m4;m5;m6;m7;m8;m9;m10;m11]``;
+*)
+
+val _ = export_theory();
